Add files via upload

Project_Perl.v
@@ -1,8 +1,9 @@
-Inductive Var := n | x | y | z.
+Inductive Var := n | x | y | z | s | k.
 
 Scheme Equality for Var.
 
 Definition Env := Var -> nat.
+
 
 Definition env : Env :=
   fun x =>
@@ -37,26 +38,18 @@ Notation "A *' B" := (amul A B) (at level 46).
 Notation "A %' B" := (amod A B) (at level 46).
 Notation "A /' B" := (adiv A B) (at level 46).
 
-Inductive BExp :=
-| btrue : BExp
-| bfalse : BExp
-| bequal : AExp -> AExp -> BExp
-| blessthan : AExp -> AExp -> BExp
-| bnot : BExp -> BExp
-| band : BExp -> BExp -> BExp
-| bor : BExp -> BExp -> BExp.
+Require Import Coq.Arith.PeanoNat.
 
-Notation "!' A" := (bnot A)(at level 53).
-Notation "A == B" := (bequal A B) (at level 51).
-Notation "A != B" := (bnot(A == B)) (at level 51).
-Notation "A &&' B" := (band A B) (at level 51).
-Notation "A ||' B" := (bor A B) (at level 51).
-Notation "A <' B" := (blessthan A B) (at level 52).
-Notation "A >' B" := (bnot (A <' B)) (at level 52).
-Notation "A <=' B" := (bnot (A >' B)) (at level 52).
-Notation "A >=' B" := (bnot (A <' B)) (at level 52).
-
-
+Fixpoint aevalF (a : AExp) (env : Env) : nat :=
+  match a with
+  | avar var => env var
+  | anum v => v
+  | aplus a1 a2 => (aevalF a1 env) + (aevalF a2 env)
+  | aminus a1 a2 => (aevalF a1 env) - (aevalF a2 env)
+  | amul a1 a2 => (aevalF a1 env) * (aevalF a2 env)
+  | adiv a1 a2 => (aevalF a1 env) / (aevalF a2 env)
+  | amod a1 a2 => (aevalF a1 env) mod (aevalF a2 env)
+  end.
 
 Inductive Coada :=
 | nil_coada : Coada
@@ -69,10 +62,11 @@ Notation "(' X ')" := (const_coada X nil_coada).  (* need level *)
 
 Notation "(' x , y , .. , z ')" := (const_coada x (const_coada y .. (const_coada z nil_coada) ..)).
 
-Definition l := (' 2,4,6 ').
+Definition l1 := (' 2,4,6 ').
+Definition l2 := (' 2, 23, 38 ').
 
-Check l.
-Compute l.
+Check l2.
+Compute l2.
 
 Definition C_first (l:Coada) : AExp :=
   match l with
@@ -80,7 +74,7 @@ Definition C_first (l:Coada) : AExp :=
     | v :: _ => v
   end.
 
-Compute (C_first l ).
+Compute (C_first l1 ).
 
 Definition C_pop (l:Coada) : Coada :=
   match l with
@@ -88,7 +82,7 @@ Definition C_pop (l:Coada) : Coada :=
     | v :: l' => l'
   end.
 
-Compute (C_pop (l)).
+Compute (C_pop (l1)).
 
 Fixpoint append (l1 l2 : Coada) : Coada :=
   match l1 with
@@ -128,6 +122,8 @@ Definition S_push (n:AExp) (l:Stiva) : Stiva :=
     | {' '} => const_stiva n l
     | _ ':: _ => n ':: l
   end.
+
+Definition stv1 := {' 5,6 '}.
 
 Compute (S_push (5) {' 2, 3 '}).
 
@@ -183,7 +179,7 @@ Notation "open ( A, '<' , B )" := (open_read B) (at level 30).
 *)
 Inductive H_pair :=
 | n_pair : H_pair
-| c_pair : nat -> nat -> H_pair.
+| c_pair : nat -> AExp -> H_pair.
 
 Inductive Hash :=
 | null_h : Hash
@@ -214,7 +210,9 @@ Compute hash2.
 
 Import Nat.
 
-Fixpoint get_h (h:Hash) (k:nat) : nat :=
+
+
+Fixpoint get_h (h:Hash) (k:nat) : AExp :=
   match h with
     | null_h => 0
     | q :': w => match q with
@@ -229,6 +227,110 @@ Notation "H #[ X ]# " := (get_h H X) (at level 30).
 
 Compute get_h hash2 2.
 
+
+
+Reserved Notation "A =[ S ]=> N" (at level 60).
+
+Inductive aeval : AExp -> Env -> nat -> Prop :=
+| const : forall n sigma, anum n =[ sigma ]=> n  
+| var : forall v sigma, avar v =[ sigma ]=> (sigma v)
+| add : forall a1 a2 i1 i2 sigma n,
+    a1 =[ sigma ]=> i1 ->
+    a2 =[ sigma ]=> i2 ->
+    n = i1 + i2 ->
+    a1 +' a2 =[sigma]=> n
+| subst : forall a1 a2 i1 i2 sigma n,
+    a1 =[ sigma ]=> i1 ->
+    a2 =[ sigma ]=> i2 ->
+    n = i1 - i2 ->
+    a1 -' a2 =[sigma]=> n
+| times : forall a1 a2 i1 i2 sigma n,
+    a1 =[ sigma ]=> i1 ->
+    a2 =[ sigma ]=> i2 ->
+    n = i1 * i2 ->
+    a1 *' a2 =[sigma]=> n
+| div : forall a1 a2 i1 i2 sigma n,
+    a1 =[ sigma ]=> i1 ->
+    a2 =[ sigma ]=> i2 ->
+    n = i1 / i2 ->
+    a1 /' a2 =[sigma]=> n
+| modulo : forall a1 a2 i1 i2 sigma n,
+    a1 =[ sigma ]=> i1 ->
+    a2 =[ sigma ]=> i2 ->
+    n = i1 mod i2 ->
+    a1 %' a2 =[sigma]=> n
+where "a =[ sigma ]=> n" := (aeval a sigma n).
+
+Hint Constructors aeval.
+
+Inductive BExp :=
+| btrue : BExp
+| bfalse : BExp
+| bequal : AExp -> AExp -> BExp
+| blessthan : AExp -> AExp -> BExp
+| bnot : BExp -> BExp
+| band : BExp -> BExp -> BExp
+| bor : BExp -> BExp -> BExp.
+
+Notation "!' A" := (bnot A)(at level 53).
+Notation "A == B" := (bequal A B) (at level 51).
+Notation "A != B" := (bnot(A == B)) (at level 51).
+Notation "A &&' B" := (band A B) (at level 51).
+Notation "A ||' B" := (bor A B) (at level 51).
+Notation "A <' B" := (blessthan A B) (at level 52).
+Notation "A >' B" := (bnot (A <' B)) (at level 52).
+Notation "A <=' B" := (bnot (A >' B)) (at level 52).
+Notation "A >=' B" := (bnot (A <' B)) (at level 52).
+
+Fixpoint bevalF (b : BExp) (env : Env) : bool :=
+  match b with
+  | btrue => true
+  | bfalse => false
+  | bequal a1 a2 => Nat.eqb (aevalF a1 env) (aevalF a2 env)
+  | blessthan a1 a2 => Nat.leb (aevalF a1 env) (aevalF a2 env)
+  | bnot b' => negb (bevalF b' env)
+  | band b1 b2 => andb (bevalF b1 env) (bevalF b2 env)
+  | bor b1 b2 => orb (bevalF b1 env) (bevalF b2 env)
+  end.
+
+Reserved Notation "B ={ S }=> B'" (at level 70).
+
+Inductive beval : BExp -> Env -> bool -> Prop :=
+| e_true : forall sigma, btrue ={ sigma }=> true
+| e_false : forall sigma, bfalse ={ sigma }=> false
+| e_equal : forall a1 a2 i1 i2 sigma b,
+    a1 =[ sigma ]=> i1 ->
+    a2 =[ sigma ]=> i2 ->
+    b = Nat.eqb i1 i2 ->
+    a1 == a2 ={ sigma }=> b
+| e_lessthan : forall a1 a2 i1 i2 sigma b,
+    a1 =[ sigma ]=> i1 ->
+    a2 =[ sigma ]=> i2 ->
+    b = Nat.leb i1 i2 ->
+    a1 <=' a2 ={ sigma }=> b
+| e_nottrue : forall b sigma,
+    b ={ sigma }=> true ->
+    (bnot b) ={ sigma }=> false
+| e_notfalse : forall b sigma,
+    b ={ sigma }=> false ->
+    (bnot b) ={ sigma }=> true
+| e_andtrue : forall b1 b2 sigma true,
+    b1 ={ sigma }=> true ->
+    b2 ={ sigma }=> true ->
+    band b1 b2 ={ sigma }=> true
+| e_andfalse : forall b1 b2 sigma,
+    b1 ={ sigma }=> false ->
+    band b1 b2 ={ sigma }=> false 
+| e_ortrue : forall b1 b2 sigma,
+    b1 ={ sigma }=> true ->
+    bor b1 b2 ={ sigma }=> true
+| e_orfalse : forall b1 b2 sigma,
+    b1 ={ sigma }=> false ->
+    b2 ={ sigma }=> false ->
+    bor b1 b2 ={ sigma }=> false 
+where "B ={ S }=> B'" := (beval B S B').
+
+
 Inductive dec :=
 | dcd : Coada -> dec
 | dst : Stiva -> dec
@@ -241,21 +343,18 @@ Coercion darr : Arr >-> dec.
 Coercion dhs : Hash >-> dec.
 
 Inductive Stmt :=
-| AExpS : AExp -> Stmt
 | assignment : Var -> AExp -> Stmt
 | sequence : Stmt -> Stmt -> Stmt
 | if_then : BExp -> Stmt -> Stmt
 | if_then_else : BExp -> Stmt -> Stmt -> Stmt
 | unless : BExp -> Stmt -> Stmt
 | while : BExp -> Stmt -> Stmt
-| myfor : Stmt -> BExp -> Stmt -> Stmt
-| foreach : Stmt -> Stmt -> Stmt
 | cd : Coada -> Stmt
 | st : Stiva -> Stmt
 | arr : Arr -> Stmt
 | hs : Hash -> Stmt
 | declaration : dec -> Stmt -> Stmt
-| sub: Stmt -> Stmt -> Stmt.
+| sub: nat -> Stmt -> Stmt.
 
 Notation "A ::= B" := (assignment A B) (at level 90).
 Notation "S ;; S'" := (sequence S S') (at level 93, right associativity).
@@ -265,8 +364,44 @@ Coercion cd : Coada >-> Stmt.
 Coercion st : Stiva >-> Stmt.
 Coercion arr : Arr >-> Stmt.
 Coercion hs : Hash >-> Stmt.
-Coercion AExpS : AExp >-> Stmt.
 
+Reserved Notation "S -{ Sigma }-> Sigma'" (at level 60).
+Check update.
+Inductive eval : Stmt -> Env -> Env -> Prop :=
+| e_assignment: forall a i x sigma sigma',
+    a =[ sigma ]=> i ->
+    sigma' = (update sigma x i) ->
+    (x ::= a) -{ sigma }-> sigma'
+| e_seq : forall s1 s2 sigma sigma1 sigma2,
+    s1 -{ sigma }-> sigma1 ->
+    s2 -{ sigma1 }-> sigma2 ->
+    (s1 ;; s2) -{ sigma }-> sigma2
+| e_whilefalse : forall b s sigma,
+    b ={ sigma }=> false ->
+    while b s -{ sigma }-> sigma
+| e_whiletrue : forall b s sigma sigma',
+    b ={ sigma }=> true ->
+    (s ;; while b s) -{ sigma }-> sigma' ->
+    while b s -{ sigma }-> sigma'
+| e_if_false : forall b s s' sigma,
+    b ={ sigma }=> false ->
+    if_then_else b s s' -{ sigma }-> sigma
+| e_if_true : forall b s s' sigma ,
+    b ={ sigma }=> true ->
+    if_then_else b s s' -{ sigma }-> sigma
+| e_ift_true : forall b s sigma ,
+    b ={ sigma }=> true ->
+    if_then b s -{ sigma }-> sigma
+| e_sub: forall n s sigma,
+    sub n s -{ sigma }-> sigma
+| e_decl: forall dec s sigma,
+    declaration dec s -{ sigma }-> sigma
+| e_cpush: forall n l sigma,
+    C_push n l -{ sigma }-> sigma
+
+
+
+where "s -{ sigma }-> sigma'" := (eval s sigma sigma').
 
 
 Definition PROGRAM :=
@@ -274,21 +409,84 @@ Definition PROGRAM :=
   if_then(n == 5) 
   (
     v <-: ['5, 10, 26'];;
-    v [' 0 '];;
-    S_push (5) {' 2, 3 '};;
+    x ::= v [' 0 '];;
+    stv1 <-: {' 2,3 '};;
+    S_push (5) stv1;;
     hash1 <-: #' #( 2,5 )# ; #( 3,6 )# '# ;;
-    hash1 #[ 3 ]#
+    y ::= hash1 #[ 3 ]#
   );;
+
   sub (1) (
-    C_push (5) (' 2, 3 ')
+     l1 <-:(' 2, 3 ');;
+     C_push (10) l1
 );;
-  l <-: (' 2,4,6 ');;
-  x ::= C_first l;;
-  y ::= x +' 5;;
-  C_push y l
+  l2 <-: (' 2, 23, 38 ');;
+  s ::= C_first l2;;
+  k ::= s +' 5;;
+  C_push k l2
   .
 
 Check PROGRAM.
+
+Fixpoint execute (s : Stmt) (env : Env) (gas : nat) : Env :=
+  match gas with
+  | 0 => env
+  | S gas' =>   match s with
+                | assignment v aexp => update env v (aevalF aexp env)
+                | sequence S1 S2 => execute S2 (execute S1 env gas') gas'
+                | if_then cond s' => if (bevalF cond env )
+                       then execute (s') env gas'
+                       else env
+                | if_then_else cond s1 s2 => if (bevalF cond env )
+                            then execute (s1) env gas'
+                            else execute (s2) env gas'
+                | unless cond s' => if (bevalF cond env)
+                                   then execute (s') env gas'
+                                   else env
+                | while cond s' => if (bevalF cond env)
+                                   then execute (s' ;; (while cond s')) env gas'
+                                   else env
+                | cd Coada => env
+                | st Stiva => env
+                | arr Arr => env
+                | hs Hash => env
+                | declaration A B => env
+                | sub s1 s2 => execute s2 env gas'
+                end
+  end.
+
+Definition env0 := fun (var : Var) => 0.
+
+Compute (execute PROGRAM env0) 100 k.
+
+Definition state0 := fun (x : Var) => 0.
+
+Example eval_program :
+  exists state, PROGRAM -{ state0 }-> state /\ state k = 7.
+Proof.
+  eexists.
+  split.
+  -unfold PROGRAM.
+    + eapply e_seq.
+     ++ eapply e_assignment; eauto.
+     ++ eapply e_seq.
+      +++ eapply e_ift_true.
+        ++++ eapply e_equal; eauto.
+      +++ eapply e_seq.
+        ++++ eapply e_sub.
+        ++++ eapply e_seq.
+          +++++ eapply e_decl.
+          +++++ eapply e_seq.
+            ++++++ eapply e_assignment; eauto.
+                   eapply const.
+            ++++++ eapply e_seq.
+            +++++++ eapply e_assignment; eauto.
+            +++++++ eapply e_cpush.
+  -simpl. unfold update. simpl. reflexivity.
+Qed.
+
+
+
 
 
 
